progs/verif_sumarray.v
@@ -12,23 +12,34 @@ Lemma sum_Z_app:
 Proof.
   intros. induction a; simpl; omega.
 Qed.
-
+(*
 (* Beginning of the API spec for the sumarray.c program *)
 Definition sumarray_spec : ident * funspec :=
  DECLARE _sumarray
-(*  WITH a: val, sh : share, contents : list Z, size: Z*)
   FOR a: val, sh : share, contents : list Z, size: Z
-(*  PRE [ _a OF (tptr tuint), _n OF tint ]*)
   PRE [ (tptr tuint), tint ]
           PROP  (readable_share sh; 0 <= size <= Int.max_signed;
           Forall (fun x => 0 <= x <= Int.max_unsigned) contents)
-          (*LOCAL (temp _a a; temp _n (Vint (Int.repr size)))
-          SEP   (data_at sh (tarray tuint size) (map Vint (map Int.repr contents)) a)*)
           (LAMBDAx nil ([a; Vint (Int.repr size)])
           (SEP   (data_at sh (tarray tuint size) (map Vint (map Int.repr contents)) a)))
   POST [ tuint ]
         PROP () LOCAL(temp ret_temp  (Vint (Int.repr (sum_Z contents))))
            SEP (data_at sh (tarray tuint size) (map Vint (map Int.repr contents)) a).
+*)
+Definition sumarray_spec : ident * funspec :=
+ DECLARE _sumarray
+  FOR a: val, sh : share, contents : list Z, size: Z
+  PRE [ (tptr tuint), tint ]
+          PROP  (readable_share sh; 0 <= size <= Int.max_signed;
+                 Forall (fun x => 0 <= x <= Int.max_unsigned) contents)
+          PARAMS (a; Vint (Int.repr size))
+          GLOBALS () (*TODO: make this line optional, ie insert GLOBALx nil during parsing of notation.
+                          Currently, omitting the line leads to failaure of start_function, specifically of compute_close_precondition_eq *)
+          SEP   (data_at sh (tarray tuint size) (map Vint (map Int.repr contents)) a)
+  POST [ tuint ]
+        PROP () LOCAL(temp ret_temp  (Vint (Int.repr (sum_Z contents))))
+           SEP (data_at sh (tarray tuint size) (map Vint (map Int.repr contents)) a).
+Print sumarray_spec. (*Prints as LAMBDAx*)
 
 (* Note: It would also be reasonable to let [contents] have type [list int].
   Then the [Forall] would not be needed in the PROP part of PRE.
@@ -37,7 +48,6 @@ Definition sumarray_spec : ident * funspec :=
 (* The precondition of "int main(void){}" always looks like this. *)
 Definition main_spec :=
  DECLARE _main
-  (*WITH gv : globals*)
   FOR gv : globals
   PRE  [] main_pre prog tt gv
   POST [ tint ]  
